Lsharp/Paper.thy
@@ -8,9 +8,8 @@ declare [[show_question_marks=false]]
 declare [[names_short=true]]
 
 notation process_output_query ("add'_io")
-(*
-notation apart (infix "\<sharp>" 40)
-*)
+
+notation apart ("(2_ \<turnstile> _ \<sharp> _)" [50,0,50] 50)
 (*>*)
 
 text\<open>
@@ -46,9 +45,16 @@ Equality on type @{type bool} denotes logical equivalence.
 
 \<close>
 text (in Mealy) \<open>
+\section{$L^\#$}
+
 \begin{quote}
 @{datatype otree}
 \end{quote}
+Observation tree is separate data type rather than a Mealy machine.
+Get tree structure for free but need to duplicate some functionality.
+Better: conversion from \<open>otree\<close> to \<open>mealy\<close>? But currently not possible
+because \<open>mealy\<close> is total.
+
 Function @{term "orun ot is"} yields the output list of ``running'' \<open>ot\<close> on \<open>is\<close>,
 i.e. traversing \<open>ot\<close> along \<open>is\<close> and emitting the output.
 Function @{term "add_io ot is os"} extends \<open>ot\<close> such that \<open>is\<close> is mapped to \<open>os\<close>.
@@ -59,6 +65,10 @@ Function @{term "add_io ot is os"} extends \<open>ot\<close> such that \<open>is
 @{thm [mode=Rule] (sub) algo_step.intros(3)}\medskip\\
 @{thm [mode=Rule] (sub) algo_step.intros(4)}
 \end{quote}
+\begin{quote}
+@{thm [break] (sub) invar_def[unfolded sapart.simps]}
+\end{quote}
+
 \<close>
 (*<*)
 end
